Isabelle/04_Composed_operations/Complex_operation_interactions.thy
@@ -7,38 +7,11 @@ theory Complex_operation_interactions
 "Fixed_repetition"
 "Guarded_conditional"
 "If_then_else"
-"Non_atomic_concurrency"
 "Until_loop"
 "Until_support"
 begin
 section \<open>Complex operation interactions for top\<close>
 
-
-subsubsection \<open>Restriction atomic concurrency\<close>
-theorem restriction_distrib_1: "(([p\<^sub>1] \<parallel> p\<^sub>2) \<sslash>\<^sub>p C) = ([p\<^sub>1 \<sslash>\<^sub>p C] \<parallel> (p\<^sub>2 \<sslash>\<^sub>p C))"
-  oops
-
-theorem restriction_distrib_2: "([p\<^sub>1] \<parallel> p\<^sub>2) \<sslash>\<^sub>p C \<equiv>\<^sub>p (p\<^sub>1 \<sslash>\<^sub>p C ; p\<^sub>2) \<union>\<^sub>p (p\<^sub>2 \<sslash>\<^sub>p C ; p\<^sub>1)" \<comment> \<open>NEW\<close>
-  apply (auto simp: non_atomic_conc_def)
-  by (metis compose_absorb_1 restrict_distrib_3)
-
-subsubsection \<open>Restriction non-atomic concurrency\<close>
-theorem restriction_distrib_1: "([p\<^sub>1, p\<^sub>2] \<parallel> q) \<sslash>\<^sub>p C = ((q\<sslash>\<^sub>p C;p\<^sub>1);p\<^sub>2 \<union>\<^sub>p ((p\<^sub>1\<sslash>\<^sub>p C;q);p\<^sub>2)) \<union>\<^sub>p ((p\<^sub>1\<sslash>\<^sub>p C;p\<^sub>2);q)"
-  oops
-theorem restriction_distrib_2: "([p\<^sub>1, p\<^sub>2] \<parallel> q) \<sslash>\<^sub>p C \<triangleq> ((q\<sslash>\<^sub>p C;p\<^sub>1);p\<^sub>2 \<union>\<^sub>p ((p\<^sub>1\<sslash>\<^sub>p C;q);p\<^sub>2)) \<union>\<^sub>p ((p\<^sub>1\<sslash>\<^sub>p C;p\<^sub>2);q)"
-  oops
-theorem restriction_distrib_3: "([p\<^sub>1, p\<^sub>2] \<parallel> q) \<sslash>\<^sub>p C \<equiv>\<^sub>p ((q\<sslash>\<^sub>p C;p\<^sub>1);p\<^sub>2 \<union>\<^sub>p ((p\<^sub>1\<sslash>\<^sub>p C;q);p\<^sub>2)) \<union>\<^sub>p ((p\<^sub>1\<sslash>\<^sub>p C;p\<^sub>2);q)"
-proof -
-  have "([p\<^sub>1, p\<^sub>2] \<parallel> q) \<sslash>\<^sub>p C = (((q ; p\<^sub>1) ; p\<^sub>2 \<union>\<^sub>p (p\<^sub>1 ; q) ; p\<^sub>2) \<union>\<^sub>p (p\<^sub>1 ; p\<^sub>2) ; q) \<sslash>\<^sub>p C"
-    by (simp add: concor_three_1)
-  moreover have "... \<equiv>\<^sub>p ((q ; p\<^sub>1) ; p\<^sub>2 \<union>\<^sub>p (p\<^sub>1 ; q) ; p\<^sub>2) \<sslash>\<^sub>p C \<union>\<^sub>p ((p\<^sub>1 ; p\<^sub>2) ; q) \<sslash>\<^sub>p C" using restrict_distrib_3 by auto
-  moreover have "... \<equiv>\<^sub>p ((((q ; p\<^sub>1) ; p\<^sub>2) \<sslash>\<^sub>p C) \<union>\<^sub>p (((p\<^sub>1 ; q) ; p\<^sub>2) \<sslash>\<^sub>p C)) \<union>\<^sub>p ((p\<^sub>1 ; p\<^sub>2) ; q) \<sslash>\<^sub>p C"using restrict_distrib_3
-    by (metis compose_absorb_1 compose_absorb_3 choice_equiv)
-  moreover have "... \<equiv>\<^sub>p ((q\<sslash>\<^sub>p C;p\<^sub>1);p\<^sub>2 \<union>\<^sub>p ((p\<^sub>1\<sslash>\<^sub>p C;q);p\<^sub>2)) \<union>\<^sub>p ((p\<^sub>1\<sslash>\<^sub>p C;p\<^sub>2);q)"
-    by (metis choice_assoc_1 choice_assoc_3 compose_absorb_1)
-  ultimately show ?thesis
-    by (smt (verit, best) equiv_is_transitive)
-qed
 
 
 subsubsection \<open>Restriction guarded conditional\<close>
@@ -58,11 +31,11 @@ theorem restriction_ite: "(ITE C a b) \<sslash>\<^sub>p D \<equiv>\<^sub>p (ITE 
   by (metis restrict_distrib_3 restrict_commute)
 
 subsubsection \<open>Restriction fixed repetition\<close>
-theorem restriction_fixed_repetition_1: "0<n \<Longrightarrow> (p\<^bold>^Suc n) \<sslash>\<^sub>p C \<equiv>\<^sub>p (p \<sslash>\<^sub>p C);(p\<^bold>^n)"
+theorem restriction_fixed_repetition_1: "0<n \<Longrightarrow> (p\<^bold>^(Suc n)) \<sslash>\<^sub>p C \<equiv>\<^sub>p (p \<sslash>\<^sub>p C);(p\<^bold>^n)"
 proof -
   assume a1: "0<n"
-  from a1 fixed_rep_decomp_front have l0: "(p \<^bold>^ Suc n) \<equiv>\<^sub>p p;p \<^bold>^ n" by auto
-  from a1 have l1: "(p \<^bold>^ Suc n) \<sslash>\<^sub>p C \<equiv>\<^sub>p (p;p \<^bold>^ n) \<sslash>\<^sub>p C"
+  from a1 fixed_rep_decomp_front have l0: "(p \<^bold>^ (Suc n)) \<equiv>\<^sub>p p;p \<^bold>^ n" by auto
+  from a1 have l1: "(p \<^bold>^ (Suc n)) \<sslash>\<^sub>p C \<equiv>\<^sub>p (p;p \<^bold>^ n) \<sslash>\<^sub>p C"
     using restriction_equiv l0 by auto
   have "(p;p \<^bold>^ n) \<sslash>\<^sub>p C \<equiv>\<^sub>p ((p\<sslash>\<^sub>p C);p \<^bold>^ n)"
     using compose_absorb_3 by auto
@@ -75,33 +48,15 @@ theorem restriction_fixed_repetition_2: "is_feasible p \<Longrightarrow> (p\<^bo
   by (metis compose_absorb_1 restriction_equiv skip_compose_l_of_fixed_rep_1)
 
 theorem restriction_fixed_repetition_3:  "(p\<^bold>^n) \<sslash>\<^sub>p C \<equiv>\<^sub>p (Skip C);(p\<^bold>^n)"
-  by (simp add: Skip.skip_restrict equiv_is_symetric)
+  by (simp add: Skip_comprestrict equiv_is_symetric)
 
 subsubsection \<open>Restriction arbitrary repetition\<close>
 theorem "loop p s f \<sslash>\<^sub>p C \<equiv>\<^sub>p Skip C ; loop p s f"
-  by (simp add: equiv_is_symetric Skip.skip_restrict)
+  by (simp add: Skip_comprestrict equiv_is_symetric)
 
 subsubsection \<open>Restriction until_support\<close>
 subsubsection \<open>Restriction until\<close>
 
-
-
-subsubsection \<open>Composition atomic concurrency\<close>
-theorem composition_refines_atomic_conc_weakens: "weakens ([p\<^sub>1] \<parallel> p\<^sub>2) (p\<^sub>1;p\<^sub>2)"
-  by (simp add: non_atomic_conc_def weakens_def)
-
-theorem composition_refines_atomic_conc_strengthens: "strengthens (p\<^sub>1;p\<^sub>2) ([p\<^sub>1] \<parallel> p\<^sub>2)"
-  apply (auto simp: non_atomic_conc_def program_is_specialize_of_choice specialize_def strengthens_def)
-  by (metis UnI1 restr_post_def restrict_prop_4)
-
-theorem composition_refines_atomic_conc: "p\<^sub>1;p\<^sub>2 \<sqsubseteq>\<^sub>p ([p\<^sub>1] \<parallel> p\<^sub>2)"
-  oops
-
-theorem composition_is_specialize_of_atomic_conc: "p\<^sub>1;p\<^sub>2 \<subseteq>\<^sub>p ([p\<^sub>1] \<parallel> p\<^sub>2)"
-  by (simp add: non_atomic_conc_def program_is_specialize_of_choice)
-
-theorem commute_compose: "commute_programs3 p\<^sub>1 p\<^sub>2 \<Longrightarrow> ([p\<^sub>1] \<parallel> p\<^sub>2) \<equiv>\<^sub>p p\<^sub>1 ; p\<^sub>2"
-  by (auto simp: commute_programs3_def non_atomic_conc_def choice_def equiv_def restr_post_def composition_def restrict_r_def)
 
 subsubsection \<open>Composition non-atomic concurrency\<close>
 subsubsection \<open>Composition If-then-else\<close>
@@ -110,14 +65,6 @@ subsubsection \<open>Composition arbitrary repetition\<close>
 subsubsection \<open>Composition until_support\<close>
 subsubsection \<open>Composition until\<close>
 
-
-subsubsection \<open>Choice atomic concurrency\<close>
-theorem concur_distrib1: "[p\<^sub>1] \<parallel> (p\<^sub>2 \<union>\<^sub>p p\<^sub>3) \<equiv>\<^sub>p ([p\<^sub>1] \<parallel> p\<^sub>2) \<union>\<^sub>p ([p\<^sub>1] \<parallel> p\<^sub>3)"
-  by (simp add: concur_distrib1)
-
-theorem concur_distrib2: "([p\<^sub>2 \<union>\<^sub>p p\<^sub>3] \<parallel> p\<^sub>1) \<equiv>\<^sub>p ([p\<^sub>2] \<parallel> p\<^sub>1) \<union>\<^sub>p ([p\<^sub>3] \<parallel> p\<^sub>1)"
-  by (simp add: concur_choice1 equiv_is_reflexive)
-subsubsection \<open>Choice non-atomic concurrency\<close>
 
 subsubsection \<open>Choice guarded conditional\<close>
 theorem cond_distrib1_gc_1: "GC [(C\<^sub>1, p\<^sub>1), (C\<^sub>2, (p\<^sub>2 \<union>\<^sub>p p\<^sub>3))] \<triangleq> (GC [(C\<^sub>1, p\<^sub>1), (C\<^sub>2, p\<^sub>2)]) \<union>\<^sub>p (GC [(C\<^sub>1, p\<^sub>1), (C\<^sub>2, p\<^sub>3)])" \<comment> \<open>T48\<close>
@@ -158,15 +105,6 @@ subsubsection \<open>Choice arbitrary repetition\<close>
 subsubsection \<open>Choice until_support\<close>
 subsubsection \<open>Choice until\<close>
 
-subsubsection \<open>Corestriction atomic concurrency\<close>
-theorem corestriction_distrib: "([p\<^sub>1] \<parallel> p\<^sub>2) \<setminus>\<^sub>p C = ([p\<^sub>1 \<setminus>\<^sub>p C] \<parallel> p\<^sub>2) \<setminus>\<^sub>p C"
-  oops
-
-theorem corestriction_distributes_not_over_atomic_conc: "([p\<^sub>1] \<parallel> p\<^sub>2) \<setminus>\<^sub>p C \<equiv>\<^sub>p p\<^sub>1 ; p\<^sub>2\<setminus>\<^sub>p C  \<union>\<^sub>p p\<^sub>2 ; p\<^sub>1 \<setminus>\<^sub>p C" \<comment> \<open>NEW\<close>
-  apply (auto simp: non_atomic_conc_def)
-  by (metis corestrict_choice_3 corestrict_compose)
-
-
 subsubsection \<open>Corestriction non-atomic concurrency\<close>
 
 subsubsection \<open>Corestriction guarded conditional\<close>
@@ -188,71 +126,10 @@ subsubsection \<open>Unsafe composition fixed repetition\<close>
 subsubsection \<open>Unsafe composition arbitrary repetition\<close> 
 subsubsection \<open>Unsafe composition until_support\<close>
 subsubsection \<open>Unsafe composition until\<close>
-
 subsubsection \<open>Atomic concurrency non-atomic concurreny\<close>
-
-lemma atomic_refines_non_atomic_1: "([p\<^sub>1; p\<^sub>2] \<parallel> q) = (p\<^sub>1 ; p\<^sub>2) ; q \<union>\<^sub>p q ; (p\<^sub>1 ; p\<^sub>2)"
-  by (simp add: non_atomic_conc_def)
-
-lemma atomic_refines_non_atomic_2: "([p\<^sub>1, p\<^sub>2] \<parallel> q) = ((p\<^sub>1 ; q) ; p\<^sub>2 \<union>\<^sub>p (q ; p\<^sub>1) ; p\<^sub>2)  \<union>\<^sub>p ((p\<^sub>1 ; p\<^sub>2) ; q \<union>\<^sub>p (p\<^sub>1 ; q) ; p\<^sub>2)"
-  apply (simp add: non_atomic_conc_def)
-  by (simp add: choice_idem_2)
-
-lemma atomic_refines_non_atomic_weakens: "weakens ([p\<^sub>1, p\<^sub>2] \<parallel> q) ([p\<^sub>1; p\<^sub>2] \<parallel> q)"
-  by (auto simp: non_atomic_conc_def atomic_conc_def equal_def weakens_def)
-  
-lemma atomic_refines_non_atomic_strengthens: "strengthens ([p\<^sub>1; p\<^sub>2] \<parallel> q) ([p\<^sub>1, p\<^sub>2] \<parallel> q)"
-  by (smt (verit) atomic_refines_non_atomic_1 choice_assoc_1 choice_commute compose_assoc concor_three_1 program_is_specialize_of_choice specialize_def)
-
-theorem coarse_fine: "([p\<^sub>1; p\<^sub>2] \<parallel> q) \<sqsubseteq>\<^sub>p ([p\<^sub>1, p\<^sub>2] \<parallel> q)" \<comment> \<open>Coarse_fine\<close>
-  oops \<comment> \<open>This does not hold. When the previous lemmas hold\<close>
-
-theorem atomic_specialize_non_atomic: "([p\<^sub>1; p\<^sub>2] \<parallel> q) \<subseteq>\<^sub>p ([p\<^sub>1, p\<^sub>2] \<parallel> q)" \<comment> \<open>T56\<close>
-  by (metis atomic_refines_non_atomic_1 choice_commute compose_assoc concor_three_1 program_is_specialize_of_choice choice_safety1)
-
-theorem atomic_specialize_non_atomic_2: "([q] \<parallel> (p\<^sub>1; p\<^sub>2)) \<subseteq>\<^sub>p ([p\<^sub>1, p\<^sub>2] \<parallel> q)" \<comment> \<open>T56\<close>
-  apply (auto simp: specialize_def extends_def non_atomic_conc_def)
-  apply (metis choice_commute choice_decomp program_is_specialize_of_choice specialize_def)
-  by (metis atomic_refines_non_atomic_1 atomic_refines_non_atomic_strengthens choice_commute compose_assoc concor_three_1)
-
-
-
-theorem exchange_law1: "p\<^sub>1 ; ([p\<^sub>2] \<parallel> q) \<subseteq>\<^sub>p ([p\<^sub>1, p\<^sub>2] \<parallel> q)" \<comment> \<open>Exchange_law1\<close>
-proof -
-  have l1: "S (p\<^sub>1 ; ([p\<^sub>2] \<parallel> q)) \<subseteq> S ((p\<^sub>1 ; (p\<^sub>2; q)) \<union>\<^sub>p (p\<^sub>1 ; (q ; p\<^sub>2)))" by (auto simp: non_atomic_conc_def)
-  have l2: "S ((q ; p\<^sub>1) ; p\<^sub>2 \<union>\<^sub>p ((p\<^sub>1 ; q) ; p\<^sub>2 \<union>\<^sub>p (p\<^sub>1 ; p\<^sub>2) ; q)) \<subseteq> S ([p\<^sub>1, p\<^sub>2] \<parallel> q)" by (auto simp: non_atomic_conc_def)
-  have "p\<^sub>1 ; ([p\<^sub>2] \<parallel> q) \<equiv>\<^sub>p (p\<^sub>1 ; (p\<^sub>2; q)) \<union>\<^sub>p (p\<^sub>1 ; (q ; p\<^sub>2))" apply (auto simp: non_atomic_conc_def)
-    by (simp add: compose_distrib1_3)
-  moreover have "... \<subseteq>\<^sub>p (q ; p\<^sub>1) ; p\<^sub>2 \<union>\<^sub>p ((p\<^sub>1 ; q) ; p\<^sub>2 \<union>\<^sub>p (p\<^sub>1 ; p\<^sub>2) ; q)"
-    using program_is_specialize_of_choice by force
-  moreover have "... \<equiv>\<^sub>p [p\<^sub>1, p\<^sub>2] \<parallel> q"
-    by (metis choice_assoc_1 concor_three_1 concor_three_3)
-  ultimately show ?thesis
-    using equiv_specialize_transitivity local.l1 local.l2 by blast
-qed
-
-theorem exchange_law2: "([p\<^sub>1] \<parallel> q) ; p\<^sub>2 \<subseteq>\<^sub>p ([p\<^sub>1, p\<^sub>2] \<parallel> q)" \<comment> \<open>Exchange_law2\<close>
-proof -
-  have l1: "S (p\<^sub>1 ; ([p\<^sub>2] \<parallel> q)) \<subseteq> S (((p\<^sub>1 ; q) ; p\<^sub>2) \<union>\<^sub>p ((q ; p\<^sub>1) ; p\<^sub>2))" by (auto simp: non_atomic_conc_def)
-  have l2: "S ((q ; p\<^sub>1) ; p\<^sub>2 \<union>\<^sub>p ((p\<^sub>1 ; q) ; p\<^sub>2 \<union>\<^sub>p (p\<^sub>1 ; p\<^sub>2) ; q)) \<subseteq> S ([p\<^sub>1, p\<^sub>2] \<parallel> q)" by (auto simp: non_atomic_conc_def)
-  have "([p\<^sub>1] \<parallel> q) ; p\<^sub>2 \<equiv>\<^sub>p ((p\<^sub>1 ; q) ; p\<^sub>2) \<union>\<^sub>p ((q ; p\<^sub>1) ; p\<^sub>2)" apply (auto simp: non_atomic_conc_def)
-    by (metis compose_assoc compose_distrib2_3)
-  moreover have "... \<subseteq>\<^sub>p (q ; p\<^sub>1) ; p\<^sub>2 \<union>\<^sub>p ((p\<^sub>1 ; q) ; p\<^sub>2 \<union>\<^sub>p (p\<^sub>1 ; p\<^sub>2) ; q)"
-    using program_is_specialize_of_choice
-    by (metis choice_commute choice_safety1)
-  moreover have "... \<equiv>\<^sub>p [p\<^sub>1, p\<^sub>2] \<parallel> q"
-    by (metis choice_assoc_1 concor_three_1 concor_three_3)
-  ultimately show ?thesis
-    using equiv_specialize_transitivity local.l1 local.l2 non_atomic_conc_S non_atomic_prop1 complete_state_prop
-    by (smt (verit, ccfv_threshold) choice_state composition_state set_eq_subset sup.idem sup_commute)
-qed
-
 subsubsection \<open>Atomic concurrency inverse\<close>
 
 subsubsection \<open>Atomic concurrency guarded conditional\<close>
-theorem cond_distrib1_conc_gc: "GC [(C\<^sub>1, p\<^sub>1), (C\<^sub>2, ([p\<^sub>2] \<parallel> p\<^sub>3))] \<equiv>\<^sub>p [GC [(C\<^sub>1, p\<^sub>1), (C\<^sub>2, p\<^sub>2)]] \<parallel> GC [(C\<^sub>1, p\<^sub>1), (C\<^sub>2, p\<^sub>3)]" \<comment> \<open>Cond_distrib1\<close>
-  oops \<comment> \<open>p1;p1 can only happen right\<close>
-
 subsubsection \<open>Atomic concurrency If-then-else\<close>
 subsubsection \<open>Atomic concurrency fixed repetition\<close>
 subsubsection \<open>Atomic concurrency arbitrary repetition\<close> 
@@ -262,8 +139,6 @@ subsubsection \<open>Atomic concurrency until\<close>
 subsubsection \<open>Non-atomic concurrency inverse\<close>
 
 subsubsection \<open>Non-atomic concurrency guarded conditional\<close>
-theorem cond_distrib1_conc_ite: "(ITE C p\<^sub>1 ([p\<^sub>2] \<parallel> p\<^sub>3)) \<equiv>\<^sub>p [ITE C p\<^sub>1 p\<^sub>2] \<parallel> (ITE C p\<^sub>1 p\<^sub>3)" \<comment> \<open>Cond_distrib1\<close>
-  oops \<comment> \<open>p1;p1 can only happen right\<close>
 
 
 subsubsection \<open>Non-atomic concurrency If-then-else\<close>
