Isabelle/T_04_Composed_operations.thy
@@ -4,11 +4,10 @@ theory T_04_Composed_operations
 "04_Composed_operations/Arbitrary_repetition"
 "04_Composed_operations/Atomic_concurrency"
 "04_Composed_operations/Big_choice"
-(*"04_Composed_operations/Complex_operation_interactions"*)
+"04_Composed_operations/Complex_operation_interactions"
 "04_Composed_operations/Fixed_repetition"
 "04_Composed_operations/Guarded_conditional"
 "04_Composed_operations/If_then_else"
-(*"04_Composed_operations/Non_atomic_concurrency"*)
 "04_Composed_operations/Until_loop"
 "04_Composed_operations/Until_support"
 begin
